add "anchored product order" that I needed

theories/WF.v
@@ -12,3 +12,76 @@ HB.structure Definition WfPreorder := {A of HasWf A & Preorder A}.
 HB.structure Definition WfPoset := {A of WfPreorder A & Poset A}.
 
 Infix "≺" := mem (at level 60) : preorder_scope.
+
+(** Let (K,k) be a pointed type and let A be a well-founded poset. Obviously A^K inherits the poset structure pointwise; I want to define a well-founded order on A^k "anchored" at k using the well-founded order on K; in other words, u ≺ v iff u k ≺ v k where k is the basepoint. *)
+Module AnchoredProductOrder.
+  Section AnchoredProductOrder.
+    Parameter K : Type.
+    Parameter k : K.
+    Parameter A : WfPoset.type.
+
+    Definition multi := K → A.
+
+    Definition multi_lt (u v : multi) := ∀ x, u x ≤ v x.
+
+    Lemma multi_ltR : ∀ u, multi_lt u u.
+    Proof. by move=>?. Qed.
+
+    Lemma multi_ltT : ∀ u v w, multi_lt u v → multi_lt v w → multi_lt u w.
+    Proof.
+      move=> u v w uv vw x.
+      apply: ltT.
+      - by apply: uv.
+      - by apply: vw.
+    Qed.
+
+    HB.instance Definition _ := PreorderOfType.Build multi multi_lt multi_ltR multi_ltT.
+
+    Lemma multi_ltE : ∀ u v : multi, u ≤ v → v ≤ u → u = v.
+    Proof.
+      move=> u v uv vu.
+      apply: depfunext=> x.
+        by apply: ltE.
+    Qed.
+
+    HB.instance Definition _ := PosetOfPreorder.Build multi multi_ltE.
+
+    Definition multi_mem (u v : multi) := (u k ≺ v k) ∧ u ≤ v.
+
+    Lemma multi_memWf : well_founded multi_mem.
+    Proof.
+      move=> u.
+      move e : (u k) => uk.
+      move: uk u e.
+      apply: (well_founded_induction memWf)=> ? ih ? e.
+      constructor=>?[??].
+      apply: ih=>//=.
+      by rewrite -e.
+    Qed.
+
+    Lemma multi_memLt : ∀ u v, multi_mem u v → u ≤ v.
+    Proof. by move=>??; case. Qed.
+
+    Lemma multi_memT : ∀ u v w, multi_mem u v → multi_mem v w → multi_mem u w.
+    Proof.
+      move=> u v w [uv1 uv2] [vw1 vw2]; split.
+      - by apply: memT; eauto.
+      - by apply: ltT; eauto.
+    Qed.
+
+    Lemma multi_memL : ∀ u v w, u ≤ v → multi_mem v w → multi_mem u w.
+    Proof.
+      move=> u v w uv [vw1 vw2]; split.
+      - by apply: memL; eauto.
+      - by apply: ltT; eauto.
+    Qed.
+
+    Lemma multi_memR : ∀ u v w, multi_mem u v → v ≤ w → multi_mem u w.
+    Proof.
+      move=> u v w [uv1 uv2] vw; split.
+      - by apply: memR; eauto.
+      - by apply: ltT; eauto.
+    Qed.
+
+    HB.instance Definition _ := HasWf.Build multi multi_mem multi_memWf multi_memLt multi_memT multi_memL multi_memR.
+End AnchoredProductOrder.
